

7.1 Integration by Parts

We're going to start expanding what we can integrate. Integration can be thought of as "undoing" derivatives.

TABLE INTEGRALS \longleftrightarrow TABLE DERIVATIVES

$$\frac{d}{dx} \sin x = \cos x \longleftrightarrow \sin x + C = \int \cos x dx$$

Chain Rule \longleftrightarrow u-Substitution

$$\begin{aligned} \frac{d}{dx} f(g(x)) &= f'(g(x)) g'(x) \longleftrightarrow \int f'(g(x)) g'(x) dx \\ &= \int f'(u) du \\ &= f(g(x)) + C. \end{aligned}$$

Now we'll consider how to undo the product rule.

$$\frac{d}{dx} (fg) = f'g + fg'$$

$$\text{so } fg = \int f'g + fg' dx$$

$$fg = \int f'g dx + \int fg' dx$$

$$fg - \int f'g dx = \int fg' dx$$

$$u = f$$

$$v = g$$

$$du = f' dx$$

$$dv = g' dx$$

$$uv - \int v du = \int u dv$$

This is called integration by parts.

Ex: $\int \boxed{x} \boxed{e^x dx}$
 $\quad \quad \quad u \quad dv$

$$u = x$$

 $\quad \downarrow \text{diff}$
 $du = dx$

$$dv = e^x dx$$

 $\quad \downarrow \text{int}$
 $v = e^x$

$$= uv - \int v du$$

$$= xe^x - \int e^x dx$$

$$= xe^x - e^x + C$$

Ex: $\int x^2 e^x dx$

$$u = x^2$$
$$du = 2x dx$$

$$dv = e^x dx$$
$$v = e^x$$

$$= x^2 e^x - \int \underbrace{2x e^x dx}_{\text{again!}}$$

$$u = 2x$$
$$du = 2 dx$$

$$dv = e^x dx$$
$$v = e^x$$

$$= x^2 e^x - (2x e^x - \int 2 e^x dx)$$

$$= x^2 e^x - 2x e^x + 2e^x + C$$

How do we choose u ?

LOGARITHM
Inverse Trig
Polynomial
Exponential
Trigonometric

$$\int \ln(x) dx$$

Logarithm. (nothing else to try)

$$= x \ln(x) - \int x \left(\frac{1}{x} \right) dx$$

$$= x \ln(x) - \int dx$$

$$= x \ln(x) - x + C$$

$$u = \ln x$$

$$dv = dx$$

$$du = \frac{1}{x} dx$$

$$v = x$$

$$\int e^x \sin x dx$$

$$u = e^x$$

$$dv = \sin x dx$$

$$du = e^x dx$$

$$v = -\cos x$$

$$\begin{array}{c} \int \\ \int \\ \int \\ \int \\ \int \\ \int \end{array}$$

$$= -e^x \cos x - \int (-\cos x) e^x dx$$

$$= -e^x \cos x + \int e^x \cos x dx$$

$$u = e^x$$

$$dv = \cos x dx$$

$$= -e^x \cos x + (e^x \sin x - \int e^x \sin x dx)$$

$$du = e^x dx$$

$$v = \sin x$$

$$= -e^x \cos x + e^x \sin x - \int e^x \sin x dx$$

$$\int e^x \sin x dx = -e^x \cos x + e^x \sin x - \int e^x \sin x dx$$

I

I

$$2 \int e^x \sin x dx = -e^x \cos x + e^x \sin x$$

$$\int e^x \sin x dx = -\frac{1}{2}e^x \cos x + \frac{1}{2}e^x \sin x + C$$